---
title: "基础数学-三角函数"
date: 2020-11-25T05:24:48+08:00
draft: false
categories: ["数学"]
tags: ["基础数学", "三角函数"]
markup: pandoc
---

# 基础数学-三角函数

#### 诱导公式 

| **公式一**                                                   | **公式二**                                                   |
| ------------------------------------------------------------ | ------------------------------------------------------------ |
| sin（2kπ+α）=sin α<br />cos（2kπ+α）=cos α<br />tan（2kπ+α）=tan α<br />cot（2kπ+α）=cot α<br />sec（2kπ+α）=sec α<br />csc（2kπ+α）=csc α | sin（π+α）=-sin α<br />cos（π+α）=-cos α<br />tan（π+α）=tan α<br />cot（π+α）=cot α<br />sec（π+α）=-sec α<br />csc（π+α）=-csc α |
| 公式三                                                       | **公式四**                                                   |
| sin（-α）=-sin α<br />cos（-α）=cos α<br />tan（-α）=-tan α<br />cot（-α）=-cot α<br />sec（-α）=sec α<br />csc（-α）=-csc α | sin（π-α）=sin α<br />cos（π-α）=-cos α<br />tan（π-α）=-tan α<br />cot（π-α）=-cot α<br />sec（π-α）=-sec α<br />csc（π-α）=csc α |
| 公式五                                                       | 公式六                                                       |
| sin（α-π）=-sin α<br />cos（α-π）=-cos α<br />tan（α-π）=tan α<br />cot（α-π）=cot α<br />sec（α-π）=-sec α<br />csc（α-π）=-csc α | sin（2π-α）=-sin α<br />cos（2π-α）=cos α<br />tan（2π-α）=-tan α<br />cot（2π-α）=-cot α<br />sec（2π-α）=sec α<br />csc（2π-α）=-csc α |
| **公式七**                                                   | **公式八**                                                   |
| sin（π/2+α）=cosα<br />cos（π/2+α）=−sinα<br />tan（π/2+α）=-cotα<br />cot（π/2+α）=-tanα<br />sec（π/2+α）=-cscα<br />csc（π/2+α）=secα | sin（π/2-α）=cosα<br />cos（π/2-α）=sinα<br />tan（π/2-α）=cotα<br />cot（π/2-α）=tanα<br />sec（π/2-α）=cscα<br />csc（π/2-α）=secα |
| 公式九                                                       | **公式十**                                                   |
| sin（3π/2+α）=-cosα<br />cos（3π/2+α）=sinα<br />tan（3π/2+α）=-cotα<br />cot（3π/2+α）=-tanα<br />sec（3π/2+α）=cscα<br />csc（3π/2+α）=*-secα* | sin（3π/2-α）=-cosα<br />cos（3π/2-α）=-sinα<br />tan（3π/2-α）=cotα<br />cot（3π/2-α）=tanα<br />sec（3π/2-α）=-cscα<br />csc（3π/2-α）=-secα |

#### 倍角公式

$\begin{aligned} \sin 2 \alpha &=2 \sin \alpha \cdot \cos \alpha \\ \cos 2 \alpha &=\cos ^{2} \alpha-\sin ^{2} \alpha=2 \cos ^{2} \alpha-1=1-2 \sin ^{2} \alpha \\ \tan 2 \alpha &=\frac{2 \tan \alpha}{1-\tan ^{2} \alpha} \end{aligned}$

#### 半角公式

$\sin ^{2} \frac{\alpha}{2}=\frac{1-\cos \alpha}{2}$
$\cos ^{2} \frac{\alpha}{2}=\frac{1+\cos \alpha}{2}$
$\tan ^{2} \frac{\alpha}{2}=\frac{1-\cos \alpha}{1+\cos \alpha}$
$\tan \frac{\alpha}{2}=\frac{\sin \alpha}{1+\cos \alpha}=\frac{1-\cos \alpha}{\sin \alpha}=\csc \alpha-\cot \alpha$
$\cot \frac{\alpha}{2}=\frac{\sin \alpha}{1-\cos \alpha}=\frac{1+\cos \alpha}{\sin \alpha}=\csc \alpha+\cot \alpha$

#### 和角公式

$\sin (\alpha+\beta)=\sin \alpha \cdot \cos \beta+\cos \alpha \cdot \sin \beta$
$\sin (\alpha-\beta)=\sin \alpha \cdot \cos \beta-\cos \alpha \cdot \sin \beta$
$\cos (\alpha+\beta)=\cos \alpha \cdot \cos \beta-\sin \alpha \cdot \sin \beta$
$\cos (\alpha-\beta)=\cos \alpha \cdot \cos \beta+\sin \alpha \cdot \sin \beta$
$\tan (\alpha+\beta)=\frac{\tan \alpha+\tan \beta}{1-\tan \alpha \cdot \tan \beta}$
$\tan (\alpha-\beta)=\frac{\tan \alpha-\tan \beta}{1+\tan \alpha \cdot \tan \beta}$

#### 积化和差

$\sin \alpha \cos \beta=\frac{1}{2}[\sin (\alpha+\beta)+\sin (\alpha-\beta)]$
$\cos \alpha \sin \beta=\frac{1}{2}[\sin (\alpha+\beta)-\sin (\alpha-\beta)]$
$\cos \alpha \cos \beta=\frac{1}{2}[\cos (\alpha+\beta)+\cos (\alpha-\beta)]$
$\sin \alpha \sin \beta=-\frac{1}{2}[\cos (\alpha+\beta)-\cos (\alpha-\beta)]$

#### 和差化积

$\sin \alpha+\sin \beta=2 \sin \frac{\alpha+\beta}{2} \cos \frac{\alpha-\beta}{2} \cdots \cdots(1)$
$\sin \alpha-\sin \beta=2 \cos \frac{\alpha+\beta}{2} \sin \frac{\alpha-\beta}{2} \ldots \ldots$
$\cos \alpha+\cos \beta=2 \cos \frac{\alpha+\beta}{2} \cos \frac{\alpha-\beta}{2} \cdots \cdots(3)$
$\cos \alpha-\cos \beta=-2 \sin \frac{\alpha+\beta}{2} \sin \frac{\alpha-\beta}{2} \ldots \ldots(4)$
$\tan \alpha+\tan \beta=\frac{\sin (\alpha+\beta)}{\cos \alpha \cos \beta} \cdots \cdots(5)$
$\tan \alpha-\tan \beta=\frac{\sin (\alpha-\beta)}{\cos \alpha \cos \beta} \cdots \cdots(6)$
$\cot \alpha+\cot \beta=\frac{\sin (\alpha+\beta)}{\sin \alpha \sin \beta} \cdots \cdots(7)$
$\cot \alpha-\cot \beta=-\frac{\sin (\alpha-\beta)}{\sin \alpha \sin \beta} \cdots \cdots(8)$
$\tan \alpha+\cot \beta=\frac{\cos (\alpha-\beta)}{\cos \alpha \sin \beta} \cdots \cdots(9)$
$\tan \alpha-\cot \beta=-\frac{\cos (\alpha+\beta)}{\cos \alpha \sin \beta} \cdots \cdots(10)$

### 万能公式

$\sin a=\frac{2 \tan \frac{a}{2}}{1+\tan ^{2} \frac{a}{2}}$
$\cos a=\frac{1-\tan ^{2} \frac{a}{2}}{1+\tan ^{2} \frac{a}{2}}$
$\tan a=\frac{2 \tan \frac{a}{2}}{1-\tan ^{2} \frac{a}{2}}$

$\cot \alpha=\frac{1-\tan ^{2} \frac{\alpha}{2}}{2 \tan \frac{\alpha}{2}}$
$\sec \alpha=\frac{1+\tan ^{2} \frac{\alpha}{2}}{1-\tan ^{2} \frac{\alpha}{2}}$
$\csc \alpha=\frac{1+\tan ^{2} \frac{\alpha}{2}}{2 \tan \frac{\alpha}{2}}$